spec/bvop/bv256_op.s.dfy
@@ -61,11 +61,6 @@ module bv256_op_s refines bv_op_s
         ensures (num_bytes == 16 && x < integers.BASE_128) ==> (r == x * integers.BASE_128);
         ensures (num_bytes == 24 && x < integers.BASE_64) ==> (r == x * integers.BASE_192);
 
-    function method {:opaque} msb(x: uint): uint1
-    {
-        if ((x as bv256 >> 255) & 1 == 1) then 1 else 0
-    }
-
     function method {:opaque} eighth_split(x: uint, sel: nat): integers.uint32
         requires 0 <= sel <= 7
     {
